\documentclass[11pt,largemargins]{homework}
\newcommand{\R}{\mathbb{R}}
\newcommand{\N}{\mathbb{N}}
\newcommand{\Q}{\mathbb{Q}}
\newcommand{\Z}{\mathbb{Z}}
\newcommand{\ran}{\operatorname{ran}}
\newcommand{\dom}{\operatorname{dom}}
\newcommand{\eps}{\varepsilon}
\newcommand{\ssd}{\bigtriangleup}
\newcommand{\pow}{\mathcal{P}}
\usepackage{qtree}
\usepackage{commath}

% TODO: replace these with your information
% TODO: replace these with your information
\newcommand{\hwname}{Evan Fox}
\newcommand{\hwemail}{efox20@uri.edu}
\newcommand{\hwtype}{Quiz}
\newcommand{\hwnum}{1}
\newcommand{\hwclass}{MTH 451}
\newcommand{\hwlecture}{}
\newcommand{\hwsection}{}

\begin{document}
\maketitle

\question
We have that $\sigma_{XY} = E(XY) -E(X)E(Y) $ and $E(X) = \sum_{x \in X} x f_X(x)$. We calculate the marginals for $X$ and $Y$ first. 

\[f_X(0) = \frac{6}{23},f_X(1) = \frac{10}{23}, f_X(2) = \frac{5}{23}, f_X(3) = \frac{2}{23} \]

and 

\[ f_Y(0) = \frac{10}{23}, f_Y(1) = \frac{10}{23}, f_Y(2) = \frac{3}{23}, \]

so then 

\[E(X) = 0 * \frac{6}{23} + 1 * \frac{10}{23} + 2 * \frac{5}{23} + 3*\frac{2}{23} = \frac{26}{23} \] 

and 
\[E(Y) = 0 * \frac{10}{23} + 1 * \frac{10}{23} + 2 * \frac{3}{23} = \frac{16}{23} \] 

Then we have $E(XY) = \sum \sum_{(x, y) \in S} xyf(x, y)$. Note there is no positive contribution from any point containg a zero and 
hence we only need to consider $\{(1,1), (1,2), (2,1) \}$. Then 

\[E(XY) = 1*1*\frac{5}{23} +  1*2*\frac{2}{23} +  1*2*\frac{1}{23} = \frac{11}{23} \] 

Then $\sigma_{XY} = \frac{11}{23} - \frac{26}{23}(\frac{16}{23}) = -17.6 $. 

\question
Since we have that independant random variables have a covarience of 0, $X$ and $Y$ cannot be independant since they have 
a non zero covarience. 

\question 
$E(X | Y = 1) = \sum_{x \in X} x f_{X|Y}(x | 1)$. We first find $f_{X|Y}(x |1)$.

\[f_{X|Y}(x |1) = \frac{f(x, 1)}{f_Y(1)} = \frac{f(x, 1)}{\frac{10}{23}} = \frac{23}{10}f(x, 1) \] 

then 

\[E(x |Y = 1) = \tfrac{23}{10}[0*f(0,1) + 1*f(1,1) + 2*f(2,1) ] = \frac{9}{10} \] 

\question 
We have $V(X | Y = 1) = E(x^2 | Y = 1) - E(x | Y = 1)^2$. We have the first moment from the previous calculation, now we compute 
the second moment. 

\[ E(x^2 | Y = 1) = \sum_{x \in X} x^2 f_{X|Y}(x, 1) = I \] 

We already have $f_{X|Y}(x, 1) = \frac{23}{10}f(x, 1)$. So

\[ I =\tfrac{23}{10}[0^2*f(0,1) + 1^2*f(1,1) + 2^2*f(2,1)] = \frac{13}{10}   \] 

Then using the short-cut formula for conditional varience we get 

\[V(x | Y = 1) = \frac{13}{10} - \frac{9^2}{10} = \frac{13}{10} - \frac{81}{10} = \frac{-68}{10}\]


\end{document}