\documentclass[11pt,largemargins]{homework}
\newcommand{\R}{\mathbb{R}}
\newcommand{\N}{\mathbb{N}}
\newcommand{\Q}{\mathbb{Q}}
\newcommand{\Z}{\mathbb{Z}}
\newcommand{\ran}{\operatorname{ran}}
\newcommand{\dom}{\operatorname{dom}}
\newcommand{\eps}{\varepsilon}
\newcommand{\ssd}{\bigtriangleup}
\newcommand{\pow}{\mathcal{P}}

% TODO: replace these with your information
% TODO: replace these with your information
\newcommand{\hwname}{Evan Fox}
\newcommand{\hwemail}{efox20@uri.edu}
\newcommand{\hwtype}{Homework}
\newcommand{\hwnum}{1}
\newcommand{\hwclass}{MTH 316}
\newcommand{\hwlecture}{}
\newcommand{\hwsection}{}

\begin{document}
\maketitle

\question
Let $G$ be a group such that for all $g \in G$, $g^2 = e$. Prove $G$ is Abelian

\begin{proof}
    Let $g \in G$. Then $g^2 = e$ so $g = g^{-1}$; it follows that 
    every element of $G$ is it's own inverse. So for $a, b \in G$ we have 
    by closure that $ab \in G$. Thus 
    \[ ab = (ab)^{-1} = b^{-1}a^{-1} \]
    by the socks-shoes property. But then since $g = g^{-1}$ for all $g \in G$
    \[ab = b^{-1}a^{-1} = ba \]
\end{proof}

\question
Let $G$ be Abelian and define 

\[H = \{ g \in G | g^4 = e \}\] 

Prove $H \leq G$. 

\begin{proof}
    Note $e \in G$ and $e^4 = e$ so $e \in H$. Then using the two step subgroup test we show $H \leq G$. 
    So let $a, b \in H$, then $a^4 = e$ and $b^4 = e$. Since $G$ is Abelian we have 
    \[ (ab)^4 = a^4b^4 = ee = e \] 
    so $ab \in H$. Now we must show $b^{-1} \in H$ whenever $b \in H$. Note 
    \[b^4b^{-4} = b^{4-4} = b^0 = e \]
    so 
    \[e = b^4b^{-4} = eb^{-4} = b^{-4} = (b^{-1})^4\] 
    Hence $b^{-1} \in H$. So by the two step subgroup test $H \leq G$. 
\end{proof}




\end{document}